IMLTT/typed/checked/Elaboration.lean
@@ -1,4 +1,3 @@
-import Std.Tactic.BVDecide
 import IMLTT.untyped.AbstractSyntax
 import IMLTT.typed.checked.TypeChecker
 import IMLTT.typed.AnnotatedSyntax
@@ -27,89 +26,92 @@ def getFinIdx? (cx : ElabCtx) (name : Name) : Option ((n : Nat) × (Fin n)) :=
 
 end ElabCtx
 
-partial def elabATm (cx : ElabCtx): TSyntax `atm → TermElabM Q((n : Nat) × ATm n)
+partial def elabATm (cx : ElabCtx): TSyntax `atm → TermElabM ((n : Nat) × ATm n)
   | `(atm| $id:ident) => do
     let id := id.getId
     if let some ⟨n, i⟩ := cx.getFinIdx? id then
-      return q(⟨$n, ATm.var $i⟩)
+      return ⟨n, ATm.var i⟩
     else
       throwError "Unexpected identifier {id}, not in context"
   | `(atm| ($t:atm)) => elabATm cx t
   -- types
   | `(atm| 𝟘) => do
     let n : Nat := cx.length
-    return q(⟨$n, ATm.empty⟩)
+    return ⟨n, .empty⟩
   | `(atm| 𝟙) => do
     let n : Nat := cx.length
-    return q(⟨$n, .unit⟩)
+    return ⟨n, .unit⟩
   | `(atm| 𝒩) => do
     let n : Nat := cx.length
-    return q(⟨$n, .nat⟩)
+    return ⟨n, .nat⟩
   | `(atm| 𝒰) => do
     let n : Nat := cx.length
-    return q(⟨$n, .univ⟩)
+    return ⟨n, .univ⟩
   | `(atm| Π ($id:ident : $A:atm; $B:atm)) => do
-    let ~q(⟨$n, $AE⟩) ← elabATm cx A
-      | throwErrorAt A "Expected a type"
+    let ⟨n, AE⟩ ← elabATm cx A
     let id' := id.getId
-    let ~q(⟨$n', $BE⟩) ← elabATm (cx.extend id') B
-      | throwErrorAt B "Expected a type"
-    if ← isDefEq q($n') q($n+1) then
-      let piE : Q(ATm $n) := mkApp3 (mkConst ``ATm.pi) n AE BE
-      return q(⟨$n, $piE⟩)
+    let ⟨n', BE⟩ ← elabATm (cx.extend id') B
+    --if ← isDefEq q($n') q($n+1) then
+    if h : n+1 = n' then
+      let bbE : (ATm (n+1)) := by
+        rw [h]
+        exact BE
+      let piE : (ATm n) := ATm.pi AE bbE
+      return ⟨n, piE⟩
     else
       throwErrorAt B m!"Context length mismatch: expected {n'}+1, got {n}"
   --terms
   | `(atm| ⋆) => do
     let n : Nat := cx.length
-    return q(⟨$n, .tt⟩)
+    return ⟨n, .tt⟩
   | `(atm| 𝓏) => do
     let n : Nat := cx.length
-    return q(⟨$n, .zeroNat⟩)
+    return ⟨n, .zeroNat⟩
   | `(atm| 𝓈($t:atm)) => do
-    let ~q(⟨$n, $t⟩) ← elabATm cx t
-      | throwErrorAt t "Expected a term of type Nat"
-    return q(⟨$n, .succNat $t⟩)
+    let ⟨n, t⟩ ← elabATm cx t
+    return ⟨n, .succNat t⟩
   | `(atm| λ ($id:ident : $A:atm). $b:atm) => do
-    let ~q(⟨$n, $AE⟩) ← elabATm cx A
-      | throwErrorAt A "Expected a type"
+    let ⟨n, AE⟩ ← elabATm cx A
     let id' := id.getId
-    let ~q(⟨$n', $bE⟩) ← elabATm (cx.extend id') b
-      | throwErrorAt b "Expected a term"
-    if ← isDefEq q($n') q($n+1) then -- this check is for a better error
-      let lamE : Q(ATm $n) := mkApp3 (mkConst ``ATm.lam) n AE bE
-      return q(⟨$n, $lamE⟩)
+    let ⟨n', bE⟩ ← elabATm (cx.extend id') b
+    if h : n+1 = n' then
+      let bbE : (ATm (n+1)) := h ▸ bE
+      let lamE : (ATm n) := ATm.lam AE bbE
+      return ⟨n, lamE⟩
     else
       throwErrorAt b m!"Context length mismatch: expected {n'}+1, got {n}"
   | _ => throwUnsupportedSyntax
 
-elab "[ttm|" t:atm "]" : term => elabATm [] t
+elab "[ttm|" t:atm "]" : term => do
+  let ⟨_, atm⟩ ← elabATm [] t
+  return Lean.toExpr atm
 
-example : ATm 0 := [ttm| 𝟙].2
+example : ATm 0 := [ttm| 𝟙]
 #check [ttm| λ (x : 𝟙). ⋆]
 #check [ttm| Π (x : 𝒰; x)]
 
-partial def elabACtx (cx : ElabCtx) : TSyntax `actx → TermElabM (ElabCtx × Q((n : Nat) × ACtx n))
+partial def elabACtx (cx : ElabCtx) : TSyntax `actx → TermElabM (ElabCtx × ((n : Nat) × ACtx n))
   | `(actx| ε) => do
-    return ⟨[], q(⟨0, ACtx.empty⟩)⟩
+    return ⟨[], (⟨0, ACtx.empty⟩)⟩
   | `(actx| $Γ:actx ⬝ ($id:ident : $A:atm)) => do
     let id' := id.getId
-    let ⟨cx', ~q(⟨$n, $ΓE⟩)⟩ ← elabACtx cx Γ | throwErrorAt Γ "Expected a context"
-    let ~q(⟨$n', $AE⟩) ← elabATm cx' A | throwErrorAt A "Expected a type"
-    if ← isDefEq q($n') q($n) then
-      let name := mkApp (mkConst ``String.toName) (mkStrLit id'.toString)
-      let extE : Q(ACtx ($n+1)) :=
-        mkApp4 (mkConst ``ACtx.extend) n name ΓE AE
-      return ⟨cx'.extend id', q(⟨$n+1, $extE⟩)⟩
+    let ⟨cx', ⟨n, ΓE⟩⟩ ← elabACtx cx Γ
+    let ⟨n', AE⟩ ← elabATm cx' A
+    if h : n = n' then
+      let AE' : (ATm n) := h ▸ AE
+      let extE : (ACtx (n+1)) :=
+        ACtx.extend id' ΓE AE'
+      return ⟨cx'.extend id', ⟨n+1, extE⟩⟩
     else
       throwErrorAt A m!"Term missmatch: expected context length {n'} got {n}"
   | _ => throwUnsupportedSyntax
 
 
-elab "[tcx|" Γ:actx "]" : term => elabACtx [] Γ >>= (return ·.2)
+elab "[tcx|" Γ:actx "]" : term => do
+  let ⟨_, ⟨_, actx⟩⟩ ← elabACtx [] Γ
+  return Lean.toExpr actx
 
 #check [tcx| ε]
-#check ([tcx| ε ⬝ (x : 𝟙)].1 : Nat)
 #check [tcx| ε ⬝ (x : 𝟙) ⬝ (y : 𝒰) ⬝ (z : y)]
 
 structure TTm (n : Nat) where
@@ -119,48 +121,41 @@ structure TTm (n : Nat) where
   hasType : Γ ⊢ t ∶ T
 
 partial def elabTTm (stxcx : TSyntax `actx) (stxt stxT : TSyntax `atm) : TermElabM Q((n : Nat) × TTm n) := do
-  let ⟨cx, acxq⟩ ← elabACtx [] stxcx
-  let ~q(⟨$n, $acx'⟩) := acxq
-    | throwErrorAt stxcx "Expected a context"
-  let ~q(⟨$nt, $t⟩) ← elabATm cx stxt
-    | throwErrorAt stxt "Expected a term"
-  let ~q(⟨$nT, $T⟩) ← elabATm cx stxT
-    | throwErrorAt stxt "Expected a term"
-  logInfo m!"t={t}; T={T}"
-  let tn : Q(Tm $n) := mkApp2 (mkConst ``ATm.toTm) n t
-  let Tn : Q(Tm $n) := mkApp2 (mkConst ``ATm.toTm) n T
-  let proof := q(has_type 30 ($acx').toCtx $tn $Tn)
-  let ttm? : Q(Except String (PLift (HasType ($acx').toCtx $tn $Tn))) ← whnf proof
-  match ttm? with
-  | ~q(Except.ok $p) =>
-    logInfo m!"Found proof :)"
-    --return p
-    --let p : Q($acx'.toCtx ⊢ $tn ∶ $Tn) ← whnf p
-    --let pdown : Q(($acx').toCtx ⊢ ($tn) ∶ ($Tn)) := (mkApp (mkConst ``PLift.down) p)
-    let ttm := mkApp5 (mkConst ``TTm.mk) n (← mkAppM ``ACtx.toCtx #[acx']) tn Tn (← mkAppM ``PLift.down #[p])
-    logInfo m!"Elaborated term: {ttm}"
-    return ttm
-    --return q(⟨$n, { Γ := ($acx').toCtx, t := $tn, T := $Tn, hasType := $pdown }⟩)
-  | ~q(Except.error $msg) =>
-    let msg ← Meta.reduce msg
-    throwErrorAt stxt "Type error: { msg }"
-  | m => throwErrorAt stxt m!"Could not match: {m}"
-  --let ttm? := q(infer [] $t)
-  /-
-  let ttm? : Q(Option (Σ' T, [] ⊢ $t ∶ T)) ← whnf ttm?
-  match ttm? with
-  | ~q(Option.some $p) =>
-    let p : Q(Σ' T, [] ⊢ $t ∶ T) ← whnf p
-    match p with
-    | ~q(⟨$T, $p'⟩) =>
-      return q({ Γ := [], t := $t, T := $T, hasType := $p'})
-  | _ => throwError "type-incorrect!"
-  -/
+  let ⟨cx, ⟨n, actx⟩⟩ ← elabACtx [] stxcx
+  let ⟨nt, atm⟩ ← elabATm cx stxt
+  let ⟨nT, aTm⟩ ← elabATm cx stxT
+  if h : n = nt ∧ n = nT then
+    let t : Tm n := h.left ▸ atm.toTm
+    let T : Tm n := h.right ▸ aTm.toTm
+    match has_type 30 actx.toCtx t T with
+    | Except.ok _ =>
+      let ctxE : Q(Ctx $n) := Lean.toExpr (actx.toCtx)
+      let tE : Q(Tm $n) := Lean.toExpr t
+      let TE : Q(Tm $n) := Lean.toExpr T
+      match ← whnf q(has_type 30 $ctxE $tE $TE) with
+      | mkApp _ pr =>
+        let ttm := mkApp5 (mkConst ``TTm.mk) (mkNatLit n) ctxE tE TE (← mkAppM ``PLift.down #[pr])
+        return ttm
+      | _ => throwError "Could not find proof again o.O"
+    | Except.error msg =>
+      throwErrorAt stxt "Type error: { msg }"
+  else throwErrorAt stxt m!"Context length mismatch: expected {n}, got {nt} and {nT}"
 
 elab "[tt|" cx:actx "⊢" t:atm ":" T:atm "]" : term => elabTTm cx t T
 
-#reduce has_type 30 ε ⋆ (Tm.univ)
-
 def test1 := [tt| ε ⊢ ⋆ : 𝟙]
+/-- error: Type error: is_eq_type: out of fuel 𝒰 ≡ 𝟙 -/
+#guard_msgs in
 def test2 := [tt| ε ⊢ ⋆ : 𝒰]
 def test3 := [tt| ε ⊢ 𝓈(𝓏) : 𝒩]
+
+syntax "ttheorem " ident " : " actx "⊢" atm ":" atm : command
+macro_rules
+  | `(ttheorem $id:ident : $cx:actx ⊢ $t:atm : $T:atm) => do
+    let ttm_name := Name.str id.getId "_TTm"
+    let ttm_id := mkIdent ttm_name
+    `(def $ttm_id:ident := [tt| $cx ⊢ $t : $T]
+      theorem $id : ($ttm_id).Γ ⊢ ($ttm_id).t ∶ ($ttm_id).T := ($ttm_id).hasType)
+
+ttheorem test8 : ε ⊢ ⋆ : 𝟙
+#check test8
